test/opcode_analysis.py
@@ -1,0 +1,89 @@
+"""
+Note: this is wrong as it only tests the opcodes on the top level function.
+- We need all opcodes, so we need recursive look for opcodes.
+"""
+
+
+
+import dis
+import json
+from glob import glob
+
+def analyse_opcode(files_path, supported_operations):
+    """
+    Loop through the python files under the files_path directory, and for each 
+    file compile it and get its bytecode opcode instructions. Analyse 
+    the instructions by building a dictionary that contains all instructions
+    that we don't support, and how many files they are in, and how many
+    occurencies of it exist across the different files.
+
+    Args:
+        files_path (str): Path to the dir that contains the tests files.
+        supported_operations (list str): List of supported bytecode operations.
+    
+    Returns:
+        opcode_dict (dict): A dcitionary of the form:
+            {
+                "opcode": 
+                    {
+                        "num_files": (n:int),
+                        "num_occurrences": (m:int),
+                    }
+            } 
+    """
+    python_files = glob(f'{files_path}/*.py')
+    missing_operations = {}
+    
+    for f_path in python_files:
+        
+        # Read source code 
+        f = open(f_path, 'r')
+        source_code = f.read()
+        f.close()
+        
+        # Compile code to get the code object, and disassible it
+        code_obj = compile(source_code, f_path, 'exec')
+        instructions = dis.get_instructions(code_obj.co_consts[0])
+
+        # f's not supported operations
+        f_missing_operations = {} 
+        
+        # Sort instructions
+        for instr in instructions:
+            opname = instr.opname
+            
+            if opname not in supported_operations:
+                if opname in f_missing_operations:
+                    f_missing_operations[opname]['num_occurrences'] += 1
+                
+                else:
+                    if opname in missing_operations:
+                        f_missing_operations[opname] = missing_operations[opname]
+                        f_missing_operations[opname]['num_files'] += 1
+                
+                    else:
+                        f_missing_operations[opname] = {
+                            'num_files': 1,
+                            'num_occurrences': 1
+                        }
+        
+        # Add f_missing_operations to missing_operations
+        missing_operations.update(f_missing_operations)        
+
+    return missing_operations
+
+
+
+"""
+# define hyper params
+files_path = ''
+supported_operations = []
+
+# analyse
+result_dict = analyse_opcode(
+        '',
+        supported_operations
+    )
+
+print(json.dumps(result_dict, indent=4, sort_keys=True))
+"""
