test/test.py
@@ -1,4 +1,11 @@
 def top_level():
     """Write your own code inside this function
     """
-    pass
+    # pass
+    
+    # -----------------------------------------
+    assert 1 == 2
+    
+
+
+top_level()
