src/test/Test.fst
@@ -7,58 +7,46 @@ open Utils
 open PyBuiltinObjects
 (* ---------------- *)
 
-let bc_0x7f6b9ce4b9d0 = CODE [
+let bc_0x7f5b70673710 = CODE [
   LOAD_CONST 1;
-  STORE_FAST 0;
   LOAD_CONST 2;
-  STORE_FAST 1;
+  COMPARE_OP 2;
+  POP_JUMP_IF_TRUE 12;
+  LOAD_GLOBAL 0;
+  RAISE_VARARGS 1;
   LOAD_CONST 3;
-  STORE_FAST 2;
-  LOAD_FAST 0;
-  LOAD_FAST 1;
-  BINARY_MULTIPLY ;
-  LOAD_CONST 3;
-  BINARY_MULTIPLY ;
-  STORE_FAST 3;
-  LOAD_FAST 0;
-  LOAD_FAST 1;
-  LOAD_FAST 2;
-  LOAD_FAST 3;
-  BUILD_TUPLE 4;
   RETURN_VALUE ;
 ]
 
-let consts_0x7f6b9ce4b9d0 = [
-  PYTYP(createNone());
+let consts_0x7f5b70673710 = [
+  PYTYP(createString "Write your own code inside this function
+    ");
   PYTYP(createInt 1);
   PYTYP(createInt 2);
-  PYTYP(createInt 3);
+  PYTYP(createNone());
 ]
 
-let varnames_0x7f6b9ce4b9d0 = [
-  "var_1";
-  "var_2";
-  "var_3";
-  "var_4";
+let varnames_0x7f5b70673710 = [
 ]
 
-let names_0x7f6b9ce4b9d0 = [
+let names_0x7f5b70673710 = [
+  "AssertionError";
 ]
 
-let cellvars_0x7f6b9ce4b9d0 = [
+let cellvars_0x7f5b70673710 = [
 ]
 
-let freevars_0x7f6b9ce4b9d0 = [
+let freevars_0x7f5b70673710 = [
 ]
 
-let co_0x7f6b9ce4b9d0 = {
-  co_code = bc_0x7f6b9ce4b9d0;
-  co_consts = consts_0x7f6b9ce4b9d0;
-  co_varnames = varnames_0x7f6b9ce4b9d0;
-  co_names = names_0x7f6b9ce4b9d0;
-  co_cellvars = cellvars_0x7f6b9ce4b9d0;
-  co_freevars = freevars_0x7f6b9ce4b9d0;
+let co_0x7f5b70673710 = {
+  co_code = bc_0x7f5b70673710;
+  co_consts = consts_0x7f5b70673710;
+  co_varnames = varnames_0x7f5b70673710;
+  co_names = names_0x7f5b70673710;
+  co_cellvars = cellvars_0x7f5b70673710;
+  co_freevars = freevars_0x7f5b70673710;
 }
 
-let virt_m, res = runCode_returnVM co_0x7f6b9ce4b9d0
+let virt_m, res = runCode_returnVM co_0x7f5b70673710
 let print_program_state = IO.print_string (print_program_state virt_m res)
